

التاريخ: / /

موضوع الدرس:

622

Inputs = x, y, z

$\Rightarrow 2^3 = 8$ columns

Outputs = z, c'

$\Rightarrow 2^2 = 4$ rows

$$z = x \oplus y \oplus c$$

$$c' = (x \wedge y) \vee (x \wedge c) \vee (y \wedge c)$$

Truth Table

x	y	c	z	c'
0	0	0	0	0
0	0	1	1	0
0	1	0	1	0
0	1	1	0	1
1	0	0	1	0
1	0	1	0	1
1	1	0	0	1
1	1	1	1	1

$$\text{matrix} = \begin{pmatrix} 1 & 0 & 0 & 0 & 0 & 0 & 0 & 0 \\ 0 & 0 & 0 & 1 & 0 & 1 & 1 & 0 \\ 0 & 1 & 1 & 0 & 1 & 0 & 0 & 0 \\ 0 & 0 & 0 & 0 & 0 & 0 & 0 & 1 \end{pmatrix}$$

52-9

classical gates

XOR gates $z = x \oplus y \oplus c$

$$H = \begin{pmatrix} 1 & 0 & 0 & 0 & 0 & 0 & 0 & 0 \\ 0 & 0 & 0 & 1 & 0 & 1 & 1 & 0 \\ 0 & 1 & 1 & 0 & 0 & 1 & 0 & 0 \\ 0 & 0 & 0 & 0 & 0 & 0 & 0 & 1 \end{pmatrix}$$

And, OR gates $c = xy + xc + yc$

• Code •

import numpy as np

matrix = np.zeros((4,8), dtype=int)

rows = {(0,0):0, (0,1):1, (1,0):2, (1,1):3}

col = 0

for x in (0,1):

for y in (0,1):

for c in (0,1):

$$z = (x \oplus y) \oplus c$$

$$c_out = (x \& y) \mid (x \& c) \mid (y \& c)$$

row = rows[(z, c_out)]

matrix[row, col] = 1

col += 1

print("The matrix is:")

print(matrix)

$$i) X^2 = Y^2 = Z^2 = I$$

$$\therefore X^2 = \begin{bmatrix} 0 & 1 \\ 1 & 0 \end{bmatrix}^2 = \begin{bmatrix} 0 & 1 \\ 1 & 0 \end{bmatrix} \begin{bmatrix} 0 & 1 \\ 1 & 0 \end{bmatrix} = \begin{bmatrix} 1 & 0 \\ 0 & 1 \end{bmatrix} = I \checkmark$$

$$Y^2 = \begin{bmatrix} 0 & -i \\ i & 0 \end{bmatrix} \begin{bmatrix} 0 & -i \\ i & 0 \end{bmatrix} = \begin{bmatrix} 1 & 0 \\ 0 & 1 \end{bmatrix} = I$$

$$Z^2 = \begin{bmatrix} 1 & 0 \\ 0 & -1 \end{bmatrix} \begin{bmatrix} 1 & 0 \\ 0 & -1 \end{bmatrix} = \begin{bmatrix} 1 & 0 \\ 0 & 1 \end{bmatrix} = I$$

$$ii) H = \frac{1}{\sqrt{2}} (H + Z)$$

$$\therefore H + Z = \begin{bmatrix} 0 & 1 \\ 1 & 0 \end{bmatrix} + \begin{bmatrix} 1 & 0 \\ 0 & -1 \end{bmatrix} = \begin{bmatrix} 1 & 1 \\ 1 & -1 \end{bmatrix}$$

$$X \frac{1}{\sqrt{2}} = \frac{1}{\sqrt{2}} (H + Z) = \frac{1}{\sqrt{2}} \begin{bmatrix} 1 & 1 \\ 1 & -1 \end{bmatrix} = H \checkmark$$

$$iii) X = HZH$$

$$\therefore HZ = \frac{1}{\sqrt{2}} \begin{bmatrix} 1 & 1 \\ 1 & -1 \end{bmatrix} \begin{bmatrix} 1 & 0 \\ 0 & -1 \end{bmatrix} = \frac{1}{\sqrt{2}} \begin{bmatrix} 1 & -1 \\ 1 & 1 \end{bmatrix}$$

$$\therefore HZH = \frac{1}{\sqrt{2}} \begin{bmatrix} 1 & 1 \\ 1 & -1 \end{bmatrix} \frac{1}{\sqrt{2}} \begin{bmatrix} 1 & 1 \\ 1 & -1 \end{bmatrix} = \frac{1}{2} \begin{bmatrix} |X| + (-|X|) & |X| + (-|X|-1) \\ |X| + |X| & |X| + |X|-1 \end{bmatrix} = \begin{bmatrix} 0 & 1 \\ 1 & 0 \end{bmatrix} = X \checkmark$$

$$iv) Z = HXH$$

$$\therefore HX = \frac{1}{\sqrt{2}} \begin{bmatrix} 1 & 1 \\ 1 & -1 \end{bmatrix} \begin{bmatrix} 0 & 1 \\ 1 & 0 \end{bmatrix} = \frac{1}{\sqrt{2}} \begin{bmatrix} 1 & 1 \\ -1 & 1 \end{bmatrix}$$

$$HXH = \frac{1}{\sqrt{2}} \begin{bmatrix} 1 & 1 \\ -1 & 1 \end{bmatrix} \frac{1}{\sqrt{2}} \begin{bmatrix} 1 & 1 \\ 1 & -1 \end{bmatrix} = \frac{1}{2} \begin{bmatrix} 2 & 0 \\ 0 & -2 \end{bmatrix} = \begin{bmatrix} 1 & 0 \\ 0 & -1 \end{bmatrix} = Z \checkmark$$

$$v) -1Y = HYH$$

$$\therefore HY = \frac{1}{\sqrt{2}} \begin{bmatrix} 1 & 1 \\ 1 & -1 \end{bmatrix} \begin{bmatrix} 0 & -i \\ i & 0 \end{bmatrix} = \frac{1}{\sqrt{2}} \begin{bmatrix} i & -i \\ -i & -i \end{bmatrix}$$

$$\therefore HYH = \frac{1}{\sqrt{2}} \begin{bmatrix} i & -i \\ -i & -i \end{bmatrix} \frac{1}{\sqrt{2}} \begin{bmatrix} 1 & 1 \\ 1 & -1 \end{bmatrix} = \frac{1}{2} \begin{bmatrix} 0 & +2i \\ 2i & 0 \end{bmatrix} = \begin{bmatrix} 0 & +i \\ -i & 0 \end{bmatrix} = -1Y \checkmark$$

$$vi) S = T^2$$

$$\therefore T^2 = \begin{bmatrix} 1 & 0 \\ 0 & \frac{i+1}{\sqrt{2}} \end{bmatrix}^2 = \begin{bmatrix} 1 & 0 \\ 0 & \frac{i+1}{\sqrt{2}} \end{bmatrix} \begin{bmatrix} 1 & 0 \\ 0 & \frac{i+1}{\sqrt{2}} \end{bmatrix} = \begin{bmatrix} 1 & 0 \\ 0 & i \end{bmatrix} = S \checkmark$$

$$vii) -1Y = XYX$$

$$\therefore XY = \begin{bmatrix} 0 & 1 \\ 1 & 0 \end{bmatrix} \begin{bmatrix} 0 & -i \\ i & 0 \end{bmatrix} = \begin{bmatrix} i & 0 \\ 0 & -i \end{bmatrix}$$

$$XYX = \begin{bmatrix} i & 0 \\ 0 & -i \end{bmatrix} \begin{bmatrix} 0 & 1 \\ 1 & 0 \end{bmatrix} = \begin{bmatrix} 0 & i \\ -i & 0 \end{bmatrix} = -1Y \checkmark$$